[EnvBased] : strengthen the LogRel to imply ValOf.isVal

LeanStlc/EnvBased/LogRel.lean
@@ -24,6 +24,8 @@ def ValOf (A:Typ) (v:Exp) : Prop :=
     -- ∃ Ξ, 𝓖⟦ Ξ ⟧ ∋ ξ ∧
     -- -- above is not needed as specified in
     -- -- [A Case for First-Class Environments](https://doi.org/10.1145/3689800)
+    -- -- we instead strengthen that ξ isVal syntactically
+    ξ.isVal ∧
     ∀ v, 𝓥⟦ A ⟧ ∋ v -> ξ∷v ⊩ 𝓔⟦ B ⟧ ∋ e
   | _, _ => False
 
@@ -39,12 +41,60 @@ end
 def SemTyp (Γ:Ctx) (e:Exp) (A:Typ) : Prop :=
   ∀ γ, 𝓖⟦ Γ ⟧ ∋ γ -> γ ⊩ 𝓔⟦ A ⟧ ∋ e
 
+mutual -- ValOf.isVal, EnvOf.isVal
+theorem ValOf.isVal {A v} :
+  𝓥⟦ A ⟧ ∋ v ->
+  v.isVal :=
+  fun 𝓥v => by
+  cases A <;> cases v <;> try simp [ValOf] at 𝓥v
+  case int.int => constructor
+  case unit.unit => constructor
+  case prod.pair =>
+    rename_i v1 v2
+    rcases 𝓥v with ⟨𝓥v1, 𝓥v2⟩
+    have isv1 : v1.isVal := ValOf.isVal 𝓥v1
+    have isv2 : v2.isVal := ValOf.isVal 𝓥v2
+    apply Exp.isVal.pair isv1 isv2
+  case ctx.env =>
+    rename_i ξ
+    have isξ : ξ.isVal := EnvOf.isVal 𝓥v
+    apply Exp.isVal.env isξ
+  case sum.inl =>
+    rename_i v
+    have isv : v.isVal := ValOf.isVal 𝓥v
+    apply Exp.isVal.inl isv
+  case sum.inr =>
+    rename_i v
+    have isv : v.isVal := ValOf.isVal 𝓥v
+    apply Exp.isVal.inr isv
+  case arr.clos =>
+    rename_i ξ e
+    rcases ξ <;> simp [ValOf] at 𝓥v
+    rcases 𝓥v with ⟨isξ, _⟩
+    apply Exp.isVal.clos (Exp.isVal.env isξ)
+theorem EnvOf.isVal {Γ γ} :
+  𝓖⟦ Γ ⟧ ∋ γ ->
+  γ.isVal :=
+  fun 𝓖γ => by
+  cases Γ <;> cases γ <;> try simp [EnvOf] at 𝓖γ
+  case nil.nil => constructor
+  case cons.cons =>
+    rename_i γ v
+    rcases 𝓖γ with ⟨𝓖γ, 𝓥v⟩
+    have isγ : γ.isVal := EnvOf.isVal 𝓖γ
+    have isv : v.isVal := ValOf.isVal 𝓥v
+    apply Env.isVal.cons isγ isv
+end
+
 theorem adequacy {Γ e A} {γ} :
   Γ ⊨ e ∶ A ->
   𝓖⟦ Γ ⟧ ∋ γ ->
   ∃ v,
-    𝓥⟦ A ⟧ ∋ v
+    v.isVal
+  ∧ 𝓥⟦ A ⟧ ∋ v
   ∧ γ ⊩ e ⇓ v :=
   fun wt 𝓖γ => by
   unfold SemTyp ExpOf at wt
-  apply wt _ 𝓖γ
+  rcases wt γ 𝓖γ with ⟨ v, 𝓥v, ev ⟩
+  have isv := ValOf.isVal 𝓥v
+  refine ⟨ v, isv, 𝓥v, ev ⟩
